move some invariants to break a needless low-level dependency on ARMspartan.dfy

verified/ARMspartan.dfy
@@ -316,39 +316,6 @@ function GlobalUpdate(gm: globalsmap, g:symbol, a:int, v:word): globalsmap
 }
 
 //-----------------------------------------------------------------------------
-// Useful invariants preserved by instructions
-//-----------------------------------------------------------------------------
-predicate AllMemInvariant(s:state, s':state)
-    requires ValidState(s) && ValidState(s')
-{
-    s.m == s'.m
-}
-
-predicate GlobalsInvariant(s:state, s':state)
-    requires ValidState(s) && ValidState(s')
-{
-    s.m.globals == s'.m.globals
-}
-
-predicate AddrMemInvariant(s:state, s':state)
-    requires ValidState(s) && ValidState(s')
-{
-    s.m.addresses == s'.m.addresses
-}
-
-predicate SRegsInvariant(s:state, s':state)
-    requires ValidState(s) && ValidState(s')
-{
-    s.sregs == s'.sregs && s.conf == s'.conf
-}
-
-predicate AllRegsInvariant(s:state, s':state)
-    requires ValidState(s) && ValidState(s')
-{
-    s.regs == s'.regs && SRegsInvariant(s, s')
-}
-
-//-----------------------------------------------------------------------------
 // Control Flow Lemmas
 //-----------------------------------------------------------------------------
 
